scratch-mvpoly-bench/mk.sh
@@ -1,7 +1,0 @@
-rep=$1; k=$2
-cat > T_${rep}_${k}.lean <<EOF
-import MV
-set_option maxRecDepth 100000 in
-example : ((pow${rep} (gen${rep} 3) ${k}).toListX == (P${rep}.mul (pow${rep} (gen${rep} 3) $((k/2))) (pow${rep} (gen${rep} 3) $((k-k/2)))).toListX) = true := by
-  decide +kernel
-EOF
